Consistent state of boolification---it builds!
Finished flock of theorems using new definition of wf_parser:
these live in DecodeScript.sml.

Big name change Boolify -> Encode.

Starting to encode variables.

src/Boolify/src/Encode.sig
@@ -1,7 +1,7 @@
 (* ========================================================================= *)
-(* AUTOMATICALLY WRITING BOOLIFICATION FUNCTIONS FOR DATATYPES.              *)
+(* AUTOMATIC GENERATION OF ENCODING FUNCTIONS FOR DATATYPES.                 *)
 (* Created by Joe Hurd, July 2002                                            *)
 (* Basically the same as Konrad Slind's code to generate size functions      *)
 (* ========================================================================= *)
 
-signature Boolify = sig end
+signature Encode = sig end
